dafny/Practical1.dfy
@@ -1,0 +1,108 @@
+method between (p: int, r: int)
+    returns (q: int)
+    requires ((r - p) > 1)
+    ensures (p < q < r)
+{
+    q := (p + r) / 2;
+}
+
+method MultipleReturns(x: int, y: int)
+    returns (greater: int, lesser: int)
+    requires (y > 0)
+    ensures (lesser <= x)
+    ensures (greater >= x)
+{
+    greater := x + y;
+    lesser := x - y;
+}
+
+method Triple(x: int)
+    returns (r: int)
+    ensures (r == (3 * x))
+{
+    var y := Double(x);
+    r := y + x;
+}
+
+method Double(x: int)
+    returns (r: int)
+    ensures (r == 2 * x)
+
+method Max(a: int, b: int)
+    returns (c :int)
+    ensures((c == a && a >= b) || (c == b && b >= a))
+{
+    if (a > b)
+    {
+        c := a;
+    }
+    else
+    {
+        c := b;
+    }
+}
+
+function abs(x: int): int
+{
+    if (x < 0) then -x else x
+}
+
+method TestAbs()
+{
+    var v := abs(3);
+    assert 0 <= v;
+    assert v == 3;
+}
+
+function method max_func(a: int, b: int) :int
+{
+    if (a > b) then a else b
+}
+
+
+method TestMax()
+{
+    var c := max_func(1, 2);
+    assert (c == 2);
+
+    var d := max_func(1, -2);
+    assert (d == 1);
+}
+
+method new_max(a: int, b: int)
+    returns (c: int)
+    ensures((c == a && a >= b) || (c == b && b >= a))
+{
+    return max_func(a, b);
+}
+
+function method fib(n: nat): nat
+{
+    if (n < 2)
+        then 1
+        else fib(n - 2) + fib(n -1)
+}
+
+method test_fib()
+{
+    var a := fib(3);
+    assert a == 3;
+
+    a := fib(4);
+    assert a == 5;
+}
+
+function method exp_func(m: int, n: nat): int
+{
+    if (n == 0)
+        then 1
+        else m * exp_func(m, n - 1)
+}
+
+method test_exp()
+{
+    assert exp_func(2, 0) == 1;
+    assert exp_func(2, 1) == 2;
+    assert exp_func(2, 2) == 4;
+    assert exp_func(2, 3) == 8;
+}
